AwsEncryptionSDK/src/Serialize/HeaderAuth.dfy
@@ -1,22 +1,18 @@
 // Copyright Amazon.com Inc. or its affiliates. All Rights Reserved.
 // SPDX-License-Identifier: Apache-2.0
 
-include "../../../libraries/src/Collections/Sequences/Seq.dfy"
-include "../../Generated/AwsCryptographicMaterialProviders.dfy"
-include "../../AwsCryptographicMaterialProviders/Client.dfy"
-include "../../StandardLibrary/StandardLibrary.dfy"
-include "../../Util/UTF8.dfy"
-include "./SerializableTypes.dfy"
+include "../../Model/AwsEncryptionSdkTypes.dfy"
+include "SerializableTypes.dfy"
 include "SerializeFunctions.dfy"
 include "HeaderTypes.dfy"
 include "EncryptionContext.dfy"
 include "EncryptedDataKeys.dfy"
 
 module HeaderAuth {
-  import Aws.Crypto
+  import Types = AwsEncryptionSdkTypes
+  import MPL = AwsCryptographyMaterialProvidersTypes
   import Seq
   import HeaderTypes
-  import MaterialProviders.Client
   import opened EncryptedDataKeys
   import opened EncryptionContext
   import opened SerializableTypes
@@ -75,29 +71,29 @@ module HeaderAuth {
 
   function method WriteHeaderAuthTag(
     headerAuth: AESMac,
-    suite: Client.AlgorithmSuites.AlgorithmSuite
+    suite: MPL.AlgorithmSuiteInfo
   )
-    :(ret: Result<seq<uint8>, string>)
+    :(ret: Result<seq<uint8>, Types.Error>)
   {
     match suite.messageVersion
       case 1 => Success(WriteHeaderAuthTagV1(headerAuth))
       case 2 => Success(WriteHeaderAuthTagV2(headerAuth))
-      case _ => Failure("Unexpected message version")
+      case _ => Failure(Types.AwsEncryptionSdkException( message := "Unexpected message version"))
   }
 
   function method ReadHeaderAuthTagV1(
     buffer: ReadableBuffer,
-    suite: Client.AlgorithmSuites.AlgorithmSuite
+    suite: MPL.AlgorithmSuiteInfo
   )
     :(res: ReadCorrect<AESMac>)
     ensures CorrectlyRead(buffer, res, WriteHeaderAuthTagV1)
     ensures res.Success?
     ==>
-      && |res.value.data.headerIv| == suite.encrypt.ivLength as nat
-      && |res.value.data.headerAuthTag| == suite.encrypt.tagLength as nat
+      && |res.value.data.headerIv| == GetIvLength(suite) as nat
+      && |res.value.data.headerAuthTag| == GetTagLength(suite) as nat
   {
-    var headerIv :- Read(buffer, suite.encrypt.ivLength as nat);
-    var headerAuthTag :- Read(headerIv.tail, suite.encrypt.tagLength as nat);
+    var headerIv :- Read(buffer, GetIvLength(suite) as nat);
+    var headerAuthTag :- Read(headerIv.tail, GetTagLength(suite) as nat);
 
     var auth: AESMac := HeaderTypes.HeaderAuth.AESMac(
       headerIv := headerIv.data,
@@ -109,18 +105,18 @@ module HeaderAuth {
 
   function method ReadHeaderAuthTagV2(
     buffer: ReadableBuffer,
-    suite: Client.AlgorithmSuites.AlgorithmSuite
+    suite: MPL.AlgorithmSuiteInfo
   )
     :(res: ReadCorrect<AESMac>)
     ensures CorrectlyRead(buffer, res, WriteHeaderAuthTagV2)
     ensures res.Success?
     ==>
-      && |res.value.data.headerIv| == suite.encrypt.ivLength as nat
-      && |res.value.data.headerAuthTag| == suite.encrypt.tagLength as nat
+      && |res.value.data.headerIv| == GetIvLength(suite) as nat
+      && |res.value.data.headerAuthTag| == GetTagLength(suite) as nat
   {
     // TODO: probably this hardcoded iv of all 0s will go into alg suite
-    var headerIv := seq(suite.encrypt.ivLength as int, _ => 0);
-    var headerAuthTag :- Read(buffer, suite.encrypt.tagLength as nat);
+    var headerIv := seq(GetIvLength(suite) as int, _ => 0);
+    var headerAuthTag :- Read(buffer, GetTagLength(suite) as nat);
 
     var auth: AESMac := HeaderTypes.HeaderAuth.AESMac(
       headerIv := headerIv,
@@ -133,15 +129,15 @@ module HeaderAuth {
 
   function method ReadHeaderAuthTag(
     buffer: ReadableBuffer,
-    suite: Client.AlgorithmSuites.AlgorithmSuite
+    suite: MPL.AlgorithmSuiteInfo
   )
     :(res: ReadCorrect<AESMac>)
     ensures suite.messageVersion == 1 ==> CorrectlyRead(buffer, res, WriteHeaderAuthTagV1)
     ensures suite.messageVersion == 2 ==> CorrectlyRead(buffer, res, WriteHeaderAuthTagV2)
     ensures res.Success?
     ==>
-      && |res.value.data.headerIv| == suite.encrypt.ivLength as nat
-      && |res.value.data.headerAuthTag| == suite.encrypt.tagLength as nat
+      && |res.value.data.headerIv| == GetIvLength(suite) as nat
+      && |res.value.data.headerAuthTag| == GetTagLength(suite) as nat
   {
     match suite.messageVersion
       case 1 => ReadHeaderAuthTagV1(buffer, suite)
