AwsEncryptionSDK/src/Serialize/SerializeFunctions.dfy
@@ -1,9 +1,7 @@
 // Copyright Amazon.com Inc. or its affiliates. All Rights Reserved.
 // SPDX-License-Identifier: Apache-2.0
 
-include "../../../libraries/src/Collections/Sequences/Seq.dfy"
-include "../../StandardLibrary/StandardLibrary.dfy"
-include "../../Util/UTF8.dfy"
+include "../../Model/AwsEncryptionSdkTypes.dfy"
 
 module SerializeFunctions {
   import Seq
